Lp2lc/Next/package.lean
@@ -1,2 +1,0 @@
-import «Lp2lc».Next.Util
-import «Lp2lc».Next.STLC.package
