Tests/STLC/ValDemo.lean
@@ -13,7 +13,7 @@ inductive Symbol where
 
 namespace Symbolic
 
-abbrev I : Free := { Carrier := Symbol, Data := String }
+abbrev I : Parameters := { C := Symbol, D := String }
 
 abbrev Typ := AST.Typ I
 abbrev Val := AST.Val I
